\documentclass{beamer}
\usetheme{CambridgeUS}

\setbeamertemplate{caption}[numbered]{}

\usepackage{enumitem}
\usepackage{tfrupee}
\usepackage{amsmath}
\usepackage{amssymb}
\usepackage{gensymb}
\usepackage{graphicx}
\usepackage{txfonts}

\def\inputGnumericTable{}

\usepackage[latin1]{inputenc}                                 
\usepackage{color}                                            
\usepackage{array}                                            
\usepackage{longtable}                                        
\usepackage{calc}                                             
\usepackage{multirow}                                         
\usepackage{hhline}                                           
\usepackage{ifthen}
\usepackage{caption} 
\captionsetup[table]{skip=3pt}  
\providecommand{\pr}[1]{\ensuremath{\Pr\left(#1\right)}}
\providecommand{\cbrak}[1]{\ensuremath{\left\{#1\right\}}}
\renewcommand{\thefigure}{\arabic{table}}
\renewcommand{\thetable}{\arabic{table}}                                     
                               
\title{AI1110 \\ Assignment 11}
\author{U.S.M.M TEJA \\ CS21BTECH11059}
\date{17th May 2022}


\begin{document}
	% The title page
	\begin{frame}
		\titlepage
	\end{frame}
	
	% The table of contents
	\begin{frame}{Outline}
    		\tableofcontents
	\end{frame}
	
	% The question
	\section{Question}
	\begin{frame}{question 6.49}
The random variables x and y are N(0, $\sigma$) are independent. Show that if z = \left|x-y \right| , then E(z) = $\frac{2\sigma}{\sqrt{\pi}}$ , E($Z^2$) = 2$\sigma^2$
	\end{frame}
	
	% The solution
\begin{frame}{Theory}
given that z = \left|x-y \right| and E(w) = E(x) - E(y) = 0 ,

$ \sigma_w^2 = \sigma_x^2 + \sigma_y^2 $ = 2\sigma^2

now we come to a conclusion that w is a random variable is N(0, \sqrt{2}\sigma)

 we know that \[E(\left|x^{2k+1}\right|) = 2\int_{0}^{\infty} x^{2k+1}f(x) \,dx \]
and E($x^{2k}$) = 1.3.5...(n-1)$\sigma^n$
\end{frame}

    \begin{frame}{Calculation}
    So
\begin{align}
  & E(\left|x^{2k+1}\right|) = 2\int_{0}^{\infty} x^{2k+1}f(x) dx & \\  
  & E(\left|x^{1}\right|)  = 2\int_{0}^{\infty} x^{1}f(x) dx & \\
  &  = \frac{2}{\sigma\sqrt{2\pi}}\int_{0}^{\infty} x^{1}e^{\frac{-x^2}{2\sigma^2}} dx& \\
  & = -\sqrt{2}\sigma\sqrt{\frac{2}{\pi}}(e^{\frac{-\infty^2}{2\sigma^2}} - e^{\frac{-0^2}{2\sigma^2}})  & \\
  & = \frac{2\sigma}{\pi}&
\end{align}

and for 
\begin{align}
 & E(x^2) = 1\times \sigma^2&\\
 & = (\sqrt{2}\sigma)^2 = 2\sigma^2&
    \end{align}
\end{frame}

\end{document}
